Cleanup term

term.v
@@ -43,15 +43,22 @@ Module Import SomeNotations.
   Notation "⟨ x , y , .. , z ⟩" := (some_intro .. (some_intro x y) .. z) : core_scope.
 End SomeNotations.
 
-Inductive sort {α} :=
+Definition option_bind {A B} (x: option A) (f: A → option B): option B :=
+  if x is Some x' then f x' else None.
+Infix ">>=" := option_bind (at level 30, right associativity).
+
+Definition option_then {A B} (x: option A) (y: option B): option B :=
+  if x is Some _ then y else None.
+
+Infix ">>" := option_then (at level 30, right associativity).
+
+Inductive sort :=
 | unit
 | prod (A B: sort)
 | exp (s t: sort)
-| pos (κ: α) (A: sort)
-| nec (κ: α) (A: sort)
-| eq (κ μ: α).
-
-Arguments sort: clear implicits.
+| pos (κ: string) (A: sort)
+| nec (κ: string) (A: sort)
+| eq (κ μ: string).
 
 Notation "[ A , B ]" := (exp A B).
 Infix "×" := prod (at level 50).
@@ -63,13 +70,19 @@ Infix "~" := eq (at level 90).
 
 Reserved Notation "f ∘ g" (at level 30).
 
+Definition sort_eq (x y: sort): {x = y} + {x ≠ y}.
+Proof.
+  set (s := string_dec).
+  decide equality.
+Defined.
+
 (* Strings are really dumb but I don't want to figure out two things
 at the same time *)
 
-Inductive tm {α}: Type :=
+Inductive tm: Type :=
 | var (x: string)
 
-| lam (x: string) (s: sort α) (e: tm)
+| lam (x: string) (s: sort) (e: tm)
 | app (f x: tm)
 
 | tt
@@ -78,15 +91,15 @@ Inductive tm {α}: Type :=
 | π1 (e: tm)
 | π2 (e: tm)
 
-| necessity (κ: α) (e: tm)
+| necessity (κ: string) (e: tm)
 
-| ext (κ: α) (e: tm)
+| ext (κ: string) (e: tm)
 | dup (e: tm)
 
-| box (κ: α) (e: tm)
+| box (κ: string) (e: tm)
 | bind (e0: tm) (x: string) (e1: tm)
 
-| id (κ: α)
+| id (κ: string)
 | compose (e0 e1: tm)
 | sym (e: tm)
 
@@ -98,11 +111,11 @@ Arguments tm: clear implicits.
 
 Infix "∘" := compose.
 
-Definition ctx α := string → option (sort α).
-Definition mt {α}: ctx α := λ _, None.
-Definition add {α} x τ (m: ctx α): ctx α := λ y, if string_dec x y then Some τ else m y.
+Definition ctx := string → option sort.
+Definition mt: ctx := λ _, None.
+Definition add x τ (m: ctx): ctx := λ y, if string_dec x y then Some τ else m y.
 
-Theorem add_add {α} x τ0 τ1 (m: ctx α): add x τ0 (add x τ1 m) = add x τ0 m.
+Theorem add_add x τ0 τ1 (m: ctx): add x τ0 (add x τ1 m) = add x τ0 m.
 Proof.
   extensionality y.
   unfold add.
@@ -110,7 +123,7 @@ Proof.
   all: reflexivity.
 Qed.
 
-Theorem add_comm {α} x y τ0 τ1 (m: ctx α):
+Theorem add_comm x y τ0 τ1 (m: ctx):
   x ≠ y →
  add x τ0 (add y τ1 m) = add y τ1 (add x τ0 m).
 Proof.
@@ -125,7 +138,7 @@ Qed.
 
 Reserved Notation "Γ ⊢ e ∈ τ" (at level 80).
 
-Inductive judge {α} (Γ: ctx α): tm α → sort α → Type :=
+Inductive judge (Γ: ctx): tm → sort → Type :=
 | judge_var x τ:
     Γ x = Some τ →
     Γ ⊢ var x ∈ τ
@@ -190,356 +203,385 @@ Inductive judge {α} (Γ: ctx α): tm α → sort α → Type :=
     Γ ⊢ cast_nec e0 e1 ∈ (□ κ1, τ)
 where "Γ ⊢ e ∈ τ" := (judge Γ e τ).
 
-Section infer.
-  Context {α: Type} (eq_dec: forall (κ0 κ1: α), {κ0 = κ1} + {κ0 ≠ κ1}).
+Record ofty (τ: sort) := {
+  term: tm ;
+  proof: mt ⊢ term ∈ τ ;
+}.
 
-  Definition sort_eq (x y: sort α): {x = y} + {x ≠ y}.
-  Proof.
-    decide equality.
-  Defined.
+Fixpoint infer (Γ: ctx) (e: tm): option sort :=
+  match e with
+  | var x => Γ x
 
-  Fixpoint infer (Γ: ctx α) (e: tm α): option (sort α) :=
-    match e with
-    | var x => Γ x
+  | lam x τ0 e =>
+    infer (add x τ0 Γ) e >>= λ τ1,
+    Some [τ0, τ1]
 
-    | lam x τ0 e =>
-      match infer (add x τ0 Γ) e with
-      | Some τ1 => Some [τ0, τ1]
-      | _ => None
-      end
+  | app e0 e1 =>
+    infer Γ e0 >>= λ A,
+    (if A is [τ0, τ1] then Some (τ0, τ1) else None) >>= λ '(τ0, τ1),
+    infer Γ e1 >>= λ τ0',
+    (if sort_eq τ0 τ0' then Some tt else None) >>
+    Some τ1
 
-    | app e0 e1 =>
-      match (infer Γ e0, infer Γ e1) with
-      | (Some [τ0, τ1], Some τ0') =>
-        if sort_eq τ0 τ0' then
-          Some τ1
-        else
-          None
-      | _ => None
-      end
+  | tt => Some unit
 
-    | tt => Some unit
+  | fanout e0 e1 =>
+    infer Γ e0 >>= λ τ0,
+    infer Γ e1 >>= λ τ1,
+    Some (τ0 × τ1)
 
-    | fanout e0 e1 =>
-      match (infer Γ e0, infer Γ e1) with
-      | (Some τ0, Some τ1) => Some (τ0 × τ1)
-      | _ => None
-      end
+  | π1 e =>
+    infer Γ e >>= λ A,
+    if A is (τ0 × τ1)
+    then Some τ0
+    else None
 
-    | π1 e =>
-      match infer Γ e with
-      | Some (τ0 × τ1) => Some τ0
-      | _ => None
-      end
+  | π2 e =>
+    infer Γ e >>= λ A,
+    if A is (τ0 × τ1)
+    then Some τ1
+    else None
 
-    | π2 e =>
-      match infer Γ e with
-      | Some (τ0 × τ1) => Some τ1
-      | _ => None
-      end
+  | necessity κ e =>
+    infer mt e >>= λ τ,
+    Some (□ κ, τ)
 
-    | necessity κ e =>
-      match infer mt e with
-      | Some τ => Some (□ κ, τ)
-      | _ => None
-      end
+  | ext κ e =>
+    infer Γ e >>= λ A,
+    (if A is (□ κ', τ) then Some (κ', τ) else None) >>= λ '(κ', τ),
+    (if string_dec κ κ' then Some tt else None) >>
+    Some τ
+  | dup e =>
+    infer Γ e >>= λ A,
+    (if A is (□ κ, τ) then Some (κ, τ) else None) >>= λ '(κ, τ),
+    Some (□ κ, □ κ, τ)
 
-    | ext κ e =>
-      match infer Γ e with
-      | Some (□ κ', τ) =>
-        if eq_dec κ κ' then Some τ else None
-      | _ => None
-      end
-    | dup e =>
-      match infer Γ e with
-      | Some (□ κ, τ) => Some (□ κ, □ κ, τ)
-      | _ => None
-      end
+  | box κ e =>
+    infer Γ e >>= λ τ,
+    Some (◇ κ, τ)
 
-    | box κ e =>
-      match infer Γ e with
-      | Some τ => Some (◇ κ, τ)
-      | _ => None
-      end
+  | bind e0 x e1 =>
+    infer Γ e0 >>= λ A,
+    (if A is (◇ κ0, τ0) then Some (κ0, τ0) else None) >>= λ '(κ0, τ0),
+    infer (add x τ0 Γ) e1 >>= λ B,
+    (if B is (◇ κ1, τ1) then Some (κ1, τ1) else None) >>= λ '(κ1, τ1),
+    (if string_dec κ0 κ1 then Some tt else None) >>
+    Some (◇ κ1, τ1)
 
-    | bind e0 x e1 =>
-      match infer Γ e0 with
-      | Some (◇ κ0, τ0) =>
-        match infer (add x τ0 Γ) e1 with
-        | Some (◇ κ1, τ1) =>
-          if eq_dec κ0 κ1 then Some (◇ κ1, τ1) else None
-        | _ => None
-        end
-      | _ => None
-      end
+  | id κ => Some (κ ~ κ)
+  | e0 ∘ e1 =>
+    infer Γ e0 >>= λ A,
+    infer Γ e1 >>= λ B,
+    (if A is κ1 ~ κ2 then Some (κ1, κ2) else None) >>= λ '(κ1, κ2),
+    (if B is κ0 ~ κ1' then Some (κ0, κ1') else None) >>= λ '(κ0, κ1'),
+    (if string_dec κ1 κ1' then Some tt else None) >>
+    Some (κ0 ~ κ2)
 
-    | id κ => Some (κ ~ κ)
-    | e0 ∘ e1 =>
-      match (infer Γ e0, infer Γ e1) with
-      | (Some (κ1 ~ κ2), Some (κ0 ~ κ1')) =>
-        if eq_dec κ1 κ1' then Some (κ0 ~ κ2) else None
-      | _ => None
-      end
+  | sym e =>
+    infer Γ e >>= λ A,
+    (if A is κ0 ~ κ1 then Some (κ0, κ1) else None) >>= λ '(κ0, κ1),
+    Some (κ1 ~ κ0)
 
-    | sym e =>
-      match infer Γ e with
-      | Some (κ0 ~ κ1) => Some (κ1 ~ κ0)
-      | _ => None
-      end
+  | cast_pos e0 e1 =>
+    infer Γ e0 >>= λ A,
+    infer Γ e1 >>= λ B,
+    (if A is κ0 ~ κ1 then Some (κ0, κ1) else None) >>= λ '(κ0, κ1),
+    (if B is ◇ κ0', τ then Some (κ0', τ) else None) >>= λ '(κ0', τ),
+    (if string_dec κ0 κ0' then Some tt else None) >>
+    Some (◇ κ1, τ)
 
+  | cast_nec e0 e1 =>
+    infer Γ e0 >>= λ A,
+    infer Γ e1 >>= λ B,
+    (if A is κ0 ~ κ1 then Some (κ0, κ1) else None) >>= λ '(κ0, κ1),
+    (if B is □ κ0', τ then Some (κ0', τ) else None) >>= λ '(κ0', τ),
+    (if string_dec κ0 κ0' then Some tt else None) >>
+    Some (□ κ1, τ)
+  end.
 
-    | cast_pos e0 e1 =>
-      match (infer Γ e0, infer Γ e1) with
-      | (Some (κ0 ~ κ1), Some (◇ κ0', τ)) =>
-        if eq_dec κ0 κ0' then Some (◇ κ1, τ) else None
-      | _ => None
-      end
-
-    | cast_nec e0 e1 =>
-      match (infer Γ e0, infer Γ e1) with
-      | (Some (κ0 ~ κ1), Some (□ κ0', τ)) =>
-        if eq_dec κ0 κ0' then Some (□ κ1, τ) else None
-      | _ => None
-      end
-    end.
-
-  Theorem infer_sound {Γ e τ}:
-    infer Γ e = Some τ → Γ ⊢ e ∈ τ.
-  Proof.
-    generalize dependent Γ.
-    generalize dependent τ.
-    induction e.
-    all: intros τ Γ p.
-    all: cbn in *.
-    - apply judge_var.
+Theorem infer_sound {Γ e τ}:
+  infer Γ e = Some τ → Γ ⊢ e ∈ τ.
+Proof.
+  generalize dependent Γ.
+  generalize dependent τ.
+  induction e.
+  all: intros τ Γ p.
+  all: cbn in *.
+  - apply judge_var.
+    assumption.
+  - destruct (infer (add x s Γ) e) eqn:q.
+    2: discriminate.
+    inversion p.
+    subst.
+    apply judge_lam.
+    apply IHe.
+    apply q.
+  - destruct (infer Γ e1) eqn:q1.
+    all: try discriminate.
+    cbn in *.
+    destruct s.
+    all: try discriminate.
+    cbn in *.
+    destruct (infer Γ e2) eqn:q2.
+    all: try discriminate.
+    cbn in *.
+    destruct (sort_eq s1 s).
+    all: try discriminate.
+    cbn in *.
+    inversion p.
+    subst.
+    eapply judge_app.
+    Unshelve.
+    3: apply s.
+    + apply IHe1.
+      apply q1.
+    + apply IHe2.
+      apply q2.
+  - inversion p.
+    subst.
+    apply judge_tt.
+  - destruct (infer Γ e1) eqn:q1.
+    all: try discriminate.
+    destruct (infer Γ e2) eqn:q2.
+    all: try discriminate.
+    inversion p.
+    subst.
+    apply judge_fanout.
+    + apply IHe1.
       assumption.
-    - destruct (infer (add x s Γ) e) eqn:q.
-      2: discriminate.
-      inversion p.
-      subst.
-      apply judge_lam.
-      apply IHe.
-      apply q.
-    - destruct (infer Γ e1) eqn:q1.
-      2: discriminate.
-      destruct s.
-      all: try discriminate.
-      destruct (infer Γ e2) eqn:q2.
-      all: try discriminate.
-      destruct (sort_eq s1 s).
-      all: try discriminate.
-      inversion p.
-      subst.
-      eapply judge_app.
-      Unshelve.
-      3: apply s.
-      + apply IHe1.
-        apply q1.
-      + apply IHe2.
-        apply q2.
-    - inversion p.
-      subst.
-      apply judge_tt.
-    - destruct (infer Γ e1) eqn:q1.
-      all: try discriminate.
-      destruct (infer Γ e2) eqn:q2.
-      all: try discriminate.
-      inversion p.
-      subst.
-      apply judge_fanout.
-      + apply IHe1.
-        assumption.
-      + apply IHe2.
-        assumption.
-    - destruct (infer Γ e) eqn:q.
-      all: try discriminate.
-      destruct s.
-      all: try discriminate.
-      eapply judge_π1.
-      Unshelve.
-      2: apply s2.
-      inversion p.
-      subst.
-      apply IHe.
+    + apply IHe2.
       assumption.
-    - destruct (infer Γ e) eqn:q.
-      all: try discriminate.
-      destruct s.
-      all: try discriminate.
-      eapply judge_π2.
-      Unshelve.
-      2: apply s1.
-      inversion p.
-      subst.
-      apply IHe.
+  - destruct (infer Γ e) eqn:q.
+    all: try discriminate.
+    destruct s.
+    all: try discriminate.
+    eapply judge_π1.
+    Unshelve.
+    2: apply s2.
+    inversion p.
+    subst.
+    apply IHe.
+    assumption.
+  - destruct (infer Γ e) eqn:q.
+    all: try discriminate.
+    destruct s.
+    all: try discriminate.
+    eapply judge_π2.
+    Unshelve.
+    2: apply s1.
+    inversion p.
+    subst.
+    apply IHe.
+    assumption.
+  - destruct (infer mt e) eqn:q.
+    all: try discriminate.
+    inversion p.
+    subst.
+    apply judge_necessity.
+    apply IHe.
+    assumption.
+  - destruct (infer Γ e) eqn:q.
+    all: try discriminate.
+    cbn in *.
+    destruct s.
+    all: try discriminate.
+    cbn in *.
+    destruct (string_dec κ κ0).
+    all: try discriminate.
+    cbn in *.
+    inversion p.
+    subst.
+    apply judge_ext.
+    apply IHe.
+    assumption.
+  - destruct (infer Γ e) eqn:q.
+    all: try discriminate.
+    destruct s.
+    all: try discriminate.
+    inversion p.
+    subst.
+    apply judge_dup.
+    apply IHe.
+    assumption.
+  - destruct (infer Γ e) eqn:q.
+    all: try discriminate.
+    inversion p.
+    subst.
+    apply judge_box.
+    apply IHe.
+    assumption.
+  - destruct (infer Γ e1) eqn:q1.
+    all: try discriminate.
+    cbn in *.
+    destruct s.
+    all: try discriminate.
+    cbn in *.
+    destruct (infer (add x s Γ) e2) eqn:q2.
+    all: try discriminate.
+    cbn in *.
+    destruct s0.
+    all: try discriminate.
+    cbn in *.
+    destruct (string_dec κ κ0).
+    all: try discriminate.
+    cbn in *.
+    inversion p.
+    subst.
+    eapply judge_bind.
+    Unshelve.
+    3: apply s.
+    + apply IHe1.
       assumption.
-    - destruct (infer mt e) eqn:q.
-      all: try discriminate.
-      inversion p.
-      subst.
-      apply judge_necessity.
-      apply IHe.
+    + apply IHe2.
       assumption.
-    - destruct (infer Γ e) eqn:q.
-      all: try discriminate.
-      destruct s.
-      all: try discriminate.
-      destruct (eq_dec κ κ0).
-      all: try discriminate.
-      inversion p.
-      subst.
-      apply judge_ext.
-      apply IHe.
+  - inversion p.
+    subst.
+    apply judge_id.
+  - destruct (infer Γ e1) eqn:q1.
+    all: try discriminate.
+    cbn in *.
+    destruct (infer Γ e2) eqn:q2.
+    all: try discriminate.
+    cbn in *.
+    destruct s.
+    cbn in *.
+    all: try discriminate.
+    cbn in *.
+    destruct s0.
+    all: try discriminate.
+    cbn in *.
+    destruct (string_dec κ μ0).
+    all: try discriminate.
+    cbn in *.
+    inversion p.
+    subst.
+    eapply judge_compose.
+    Unshelve.
+    3: apply μ0.
+    + apply IHe1.
       assumption.
-    - destruct (infer Γ e) eqn:q.
-      all: try discriminate.
-      destruct s.
-      all: try discriminate.
-      inversion p.
-      subst.
-      apply judge_dup.
-      apply IHe.
+    + apply IHe2.
       assumption.
-    - destruct (infer Γ e) eqn:q.
-      all: try discriminate.
-      inversion p.
-      subst.
-      apply judge_box.
-      apply IHe.
+  - destruct (infer Γ e) eqn:q.
+    all: try discriminate.
+    cbn in *.
+    destruct s.
+    all: try discriminate.
+    cbn in *.
+    inversion p.
+    subst.
+    apply judge_sym.
+    apply IHe.
+    assumption.
+  - destruct (infer Γ e1) eqn:q1.
+    all: try discriminate.
+    cbn in *.
+    destruct (infer Γ e2) eqn:q2.
+    all: try discriminate.
+    cbn in *.
+    destruct s.
+    all: try discriminate.
+    cbn in *.
+    destruct s0.
+    all: try discriminate.
+    cbn in *.
+    destruct (string_dec κ κ0).
+    all: try discriminate.
+    cbn in *.
+    inversion p.
+    subst.
+    eapply judge_cast_pos.
+    Unshelve.
+    3: apply κ0.
+    + apply IHe1.
       assumption.
-    - destruct (infer Γ e1) eqn:q1.
-      all: try discriminate.
-      destruct s.
-      all: try discriminate.
-      destruct (infer (add x s Γ) e2) eqn:q2.
-      all: try discriminate.
-      destruct s0.
-      all: try discriminate.
-      destruct (eq_dec κ κ0).
-      all: try discriminate.
-      inversion p.
-      subst.
-      eapply judge_bind.
-      Unshelve.
-      3: apply s.
-      + apply IHe1.
-        assumption.
-      + apply IHe2.
-        assumption.
-    - inversion p.
-      subst.
-      apply judge_id.
-    - destruct (infer Γ e1) eqn:q1.
-      all: try discriminate.
-      destruct s.
-      all: try discriminate.
-      destruct (infer Γ e2) eqn:q2.
-      all: try discriminate.
-      destruct s.
-      all: try discriminate.
-      destruct (eq_dec κ μ0).
-      all: try discriminate.
-      inversion p.
-      subst.
-      eapply judge_compose.
-      Unshelve.
-      3: apply μ0.
-      + apply IHe1.
-        assumption.
-      + apply IHe2.
-        assumption.
-    - destruct (infer Γ e) eqn:q.
-      all: try discriminate.
-      destruct s.
-      all: try discriminate.
-      inversion p.
-      subst.
-      apply judge_sym.
-      apply IHe.
+    + apply IHe2.
       assumption.
-    - destruct (infer Γ e1) eqn:q1.
-      all: try discriminate.
-      destruct s.
-      all: try discriminate.
-      destruct (infer Γ e2) eqn:q2.
-      all: try discriminate.
-      destruct s.
-      all: try discriminate.
-      destruct (eq_dec κ κ0).
-      all: try discriminate.
-      inversion p.
-      subst.
-      eapply judge_cast_pos.
-      Unshelve.
-      3: apply κ0.
-      + apply IHe1.
-        assumption.
-      + apply IHe2.
-        assumption.
-    - destruct (infer Γ e1) eqn:q1.
-      all: try discriminate.
-      destruct s.
-      all: try discriminate.
-      destruct (infer Γ e2) eqn:q2.
-      all: try discriminate.
-      destruct s.
-      all: try discriminate.
-      destruct (eq_dec κ κ0).
-      all: try discriminate.
-      inversion p.
-      subst.
-      eapply judge_cast_nec.
-      Unshelve.
-      3: apply κ0.
-      + apply IHe1.
-        assumption.
-      + apply IHe2.
-        assumption.
-  Defined.
+  - destruct (infer Γ e1) eqn:q1.
+    all: try discriminate.
+    cbn in *.
+    destruct (infer Γ e2) eqn:q2.
+    all: try discriminate.
+    cbn in *.
+    destruct s.
+    all: try discriminate.
+    cbn in *.
+    destruct s0.
+    all: try discriminate.
+    cbn in *.
+    destruct (string_dec κ κ0).
+    all: try discriminate.
+    inversion p.
+    subst.
+    eapply judge_cast_nec.
+    Unshelve.
+    3: apply κ0.
+    + apply IHe1.
+      assumption.
+    + apply IHe2.
+      assumption.
+Defined.
 
-  Theorem infer_complete {Γ e τ}:
-    Γ ⊢ e ∈ τ → infer Γ e = Some τ.
-    intro p.
-    induction p.
-    all: cbn in *.
-    all: auto.
-    all: try rewrite IHp.
-    all: try rewrite IHp1.
-    all: try rewrite IHp2.
-    all: try reflexivity.
-    - destruct (sort_eq τ0 τ0).
-      2: contradiction.
-      reflexivity.
-    - destruct (eq_dec κ κ).
-      2: contradiction.
-      reflexivity.
-    - destruct (eq_dec κ κ).
-      2: contradiction.
-      reflexivity.
-    - destruct (eq_dec κ1 κ1).
-      2: contradiction.
-      reflexivity.
-    - destruct (eq_dec κ0 κ0).
-      2: contradiction.
-      reflexivity.
-    - destruct (eq_dec κ0 κ0).
-      2: contradiction.
-      reflexivity.
-  Qed.
-End infer.
+Theorem infer_complete {Γ e τ}:
+  Γ ⊢ e ∈ τ → infer Γ e = Some τ.
+  intro p.
+  induction p.
+  all: cbn in *.
+  all: auto.
+  all: try rewrite IHp.
+  all: cbn in *.
+  all: try rewrite IHp1.
+  all: cbn in *.
+  all: try rewrite IHp2.
+  all: cbn in *.
+  all: try reflexivity.
+  all: cbn in *.
+  - destruct (sort_eq τ0 τ0).
+    2: contradiction.
+    reflexivity.
+  - destruct (string_dec κ κ).
+    2: contradiction.
+    reflexivity.
+  - destruct (string_dec κ κ).
+    2: contradiction.
+    reflexivity.
+  - destruct (string_dec κ1 κ1).
+    2: contradiction.
+    reflexivity.
+  - destruct (string_dec κ0 κ0).
+    2: contradiction.
+    reflexivity.
+  - destruct (string_dec κ0 κ0).
+    2: contradiction.
+    reflexivity.
+Qed.
 
-Definition includes {α} (Γ Δ: ctx α): Prop :=
+Definition typed (e: tm): if infer mt e is Some τ then ofty τ else True.
+Proof.
+  destruct (infer mt e) eqn:q.
+  - exists e.
+    apply infer_sound.
+    assumption.
+  - apply I.
+Defined.
+
+Example tt_typed: ofty unit := typed tt.
+Example id_typed A: ofty (exp A A) := typed (lam "x" A (var "x")).
+Example compose_typed: ofty _ := typed (id "κ" ∘ id "κ").
+Example id_tt: ofty _ := typed (app (lam "x" unit (var "x")) tt).
+
+Definition includes (Γ Δ: ctx): Prop :=
   ∀ x τ, Δ x = Some τ → Γ x = Some τ.
 
 Notation "Γ ⊑ Δ" := (includes Γ Δ) (at level 90).
 
-Instance include_refl α: Reflexive (@includes α).
+Instance include_refl: Reflexive includes.
 Proof.
   intros ? ? ? ?.
   auto.
 Qed.
 
-Instance include_trans α: Transitive (@includes α).
+Instance include_trans: Transitive includes.
 Proof.
   intros ? ? ? p q ? ? ?.
   unfold includes in p, q.
@@ -548,13 +590,13 @@ Proof.
   auto.
 Qed.
 
-Theorem weakest {α} {Γ: ctx α}: Γ ⊑ mt.
+Theorem weakest {Γ: ctx}: Γ ⊑ mt.
 Proof.
   intros ? ? ?.
   discriminate.
 Qed.
 
-Theorem weaken {α Γ Δ} {e: tm α} {τ}:
+Theorem weaken {Γ Δ} {e: tm} {τ}:
     Γ ⊑ Δ →
     Δ ⊢ e ∈ τ → Γ ⊢ e ∈ τ.
 Proof.
@@ -576,7 +618,7 @@ Proof.
     all: auto.
 Qed.
 
-Variant whnf {α}: tm α → Type :=
+Variant whnf: tm → Type :=
 | whnf_tt: whnf tt
 | whnf_fanout e0 e1: whnf (fanout e0 e1)
 | whnf_lam x τ e: whnf (lam x τ e)
@@ -585,7 +627,7 @@ Variant whnf {α}: tm α → Type :=
 | whnf_id κ: whnf (id κ)
 .
 
-Variant cd {α}: tm α → Type :=
+Variant cd: tm → Type :=
 | cd_app e0 e1: cd (app e0 e1)
 | cd_π1 e: cd (π1 e)
 | cd_π2 e: cd (π2 e)
@@ -598,7 +640,7 @@ Variant cd {α}: tm α → Type :=
 | cd_cast_nec e0 e1: cd (cast_nec e0 e1)
 .
 
-Lemma canonical {α} {v: tm α} {τ}:
+Lemma canonical {v: tm} {τ}:
   mt ⊢ v ∈ τ → whnf v →
   match τ with
   | unit => (v = tt: Type)
@@ -627,12 +669,11 @@ Proof.
     reflexivity.
 Defined.
 
-
 Reserved Notation "'[' x ':=' s ']' t" (at level 20).
 
 Section subst.
-  Context {α: Type} (x: string) (s: tm α).
-  Fixpoint subst (ev: tm α): tm α :=
+  Context (x: string) (s: tm).
+  Fixpoint subst (ev: tm): tm :=
     match ev with
     | var y => if string_dec x y then s else ev
 
@@ -666,8 +707,7 @@ End subst.
 
 Notation "'[' x ':=' s ']' t" := (subst x s t) .
 
-Theorem subst_type {α} {Γ x} {e0 e1: tm α} {τ0 τ1}
-   (eq_dec: forall (κ0 κ1: α), {κ0 = κ1} + {κ0 ≠ κ1}):
+Theorem subst_type {Γ x} {e0 e1: tm} {τ0 τ1}:
   add x τ1 Γ ⊢ e0 ∈ τ0 →
   mt ⊢ e1 ∈ τ1 →
   Γ ⊢ [x:=e1]e0 ∈ τ0.
@@ -684,7 +724,7 @@ Proof.
   - cbn.
     destruct (string_dec x x0) eqn:r.
     + cbn in *.
-      set (p' := infer_complete eq_dec p).
+      set (p' := infer_complete p).
       unfold add in p'.
       cbn in *.
       rewrite r in p'.
@@ -696,7 +736,7 @@ Proof.
       unfold mt in *.
       discriminate.
     + cbn in *.
-      set (p' := infer_complete eq_dec p).
+      set (p' := infer_complete p).
       unfold add in p'.
       cbn in *.
       rewrite r in p'.
@@ -706,7 +746,7 @@ Proof.
     destruct (string_dec x x0).
     + subst.
       apply judge_lam.
-      rewrite add_add in X.
+      rewrite add_add in H3.
       assumption.
     + apply judge_lam.
       apply IHe0.
@@ -715,24 +755,24 @@ Proof.
       assumption.
   - cbn.
     apply IHe0.
-    refine (weaken _ X).
+    refine (weaken _ H2).
     intros ? ? ?.
     unfold mt in *.
     discriminate.
   - cbn.
     destruct (string_dec x x0).
     + subst.
-      rewrite add_add in X0.
+      rewrite add_add in H4.
       auto.
     + apply IHe0_2.
-      rewrite add_comm in X0.
+      rewrite add_comm in H4.
       2: auto.
       auto.
 Qed.
 
 Reserved Notation "t '~>' t'" (at level 40).
 
-Inductive step {α}: tm α → tm α → Type :=
+Inductive step: tm → tm → Type :=
 | step_app_lam x τ e0 e1:
     app (lam x τ e0) e1 ~> [x:=e1]e0
 | step_bind_box κ e0 x e1:
@@ -806,14 +846,14 @@ Inductive step {α}: tm α → tm α → Type :=
 
 where "A '~>' B" := (step A B).
 
-Lemma to_cd {α} {e e': tm α}: e ~> e' → cd e.
+Lemma to_cd {e e': tm}: e ~> e' → cd e.
 Proof.
   intro s.
   induction s.
   all: constructor.
 Defined.
 
-Theorem progress {α} (e: tm α) {τ}:
+Theorem progress (e: tm) {τ}:
   mt ⊢ e ∈ τ →
   whnf e + (Σ e', e ~> e').
 Proof.
@@ -977,9 +1017,7 @@ Proof.
     auto.
 Defined.
 
-Theorem preservation {α}
-        (eq_dec: forall (κ0 κ1: α), {κ0 = κ1} + {κ0 ≠ κ1})
-        (e e': tm α) τ:
+Theorem preservation (e e': tm) τ:
     e ~> e' →
     mt ⊢ e ∈ τ →
     mt ⊢ e' ∈ τ.
@@ -992,36 +1030,36 @@ Proof.
   all: intros τ0 p.
   all: inversion p.
   all: subst.
-  - inversion X.
+  - inversion H1.
     subst.
-    apply (subst_type eq_dec X1 X0).
-  - inversion X.
+    apply (subst_type H0 H3).
+  - inversion H3.
     subst.
-    apply (subst_type eq_dec X0 X1).
-  - inversion X.
-    subst.
-    auto.
-  - inversion X.
+    apply (subst_type H4 H0).
+  - inversion H0.
     subst.
     auto.
-  - inversion X.
+  - inversion H0.
     subst.
     auto.
-  - inversion X.
+  - inversion H2.
+    subst.
+    auto.
+  - inversion H0.
     subst.
     apply judge_necessity.
     apply judge_necessity.
     auto.
-  - inversion X.
+  - inversion H0.
     subst.
     auto.
-  - inversion X.
+  - inversion H1.
     subst.
     auto.
-  - inversion X.
+  - inversion H1.
     subst.
     auto.
-  - inversion X.
+  - inversion H1.
     subst.
     auto.
   - eapply judge_bind.
@@ -1074,15 +1112,15 @@ Proof.
     all: auto.
 Defined.
 
-Inductive multistep {α} (X: tm α): tm α → Type :=
+Inductive multistep (X: tm): tm → Type :=
 | halt: multistep X X
 | andthen {Y Z}: X ~> Y → multistep Y Z → multistep X Z.
-Arguments halt {α X}.
-Arguments andthen {α X Y Z}.
+Arguments halt {X}.
+Arguments andthen {X Y Z}.
 
 Notation "A ~>* B" := (multistep A B) (at level 90).
 
-Fixpoint eval {α} (e: tm α): option (tm α) :=
+Fixpoint eval (e: tm): option tm :=
   match e with
   | app (lam x _ e0) e1 => Some ([x := e1] e0)
   | bind (box _ e0) x e1 => Some ([x := e0] e1)
@@ -1100,28 +1138,23 @@ Fixpoint eval {α} (e: tm α): option (tm α) :=
   | cast_nec (id κ) (necessity _ e) => Some (necessity κ e)
 
   | app e0 e1 =>
-    if eval e0 is Some e0'
-    then Some (app e0' e1)
-    else None
+    eval e0 >>= λ e0',
+    Some (app e0' e1)
 
   | π1 e =>
-    if eval e is Some e'
-    then Some (π1 e')
-    else None
+    eval e >>= λ e',
+    Some (π1 e')
   | π2 e =>
-    if eval e is Some e'
-    then Some (π2 e')
-    else None
+    eval e >>= λ e',
+    Some (π2 e')
 
   | ext κ e =>
-    if eval e is Some e'
-    then Some (ext κ e')
-    else None
+    eval e >>= λ e',
+    Some (ext κ e')
 
   | dup e =>
-    if eval e is Some e'
-    then Some (dup e')
-    else None
+    eval e >>= λ e',
+    Some (dup e')
 
   | e0 ∘ e1 =>
     if eval e0 is Some e0'
@@ -1149,18 +1182,3 @@ Fixpoint eval {α} (e: tm α): option (tm α) :=
 
   | _ => None
   end.
-
-CoInductive stream A := cons { hd: A ; tl: option (stream A) }.
-
-Arguments cons {A}.
-Arguments hd {A}.
-Arguments tl {A}.
-
-CoFixpoint multieval {α} (e: tm α): stream (tm α) :=
-  cons e (if eval e is Some e' then Some (multieval e') else None).
-
-Inductive evalsto {α} (X: tm α): tm α → Type :=
-| evals_id: evalsto X X
-| evals_step {Y Z}: Some Y = eval X → evalsto Y Z → evalsto X Z.
-Arguments evals_id {α X}.
-Arguments evals_step {α X Y Z}.
